
\documentclass{article}

\usepackage{color}
\usepackage{epsfig}
\usepackage{amssymb}
\usepackage{listings}
\usepackage{textpos}
\usepackage{amsmath}

\newcommand\hcancel[2][black]{\setbox0=\hbox{$#2$}%
\rlap{\raisebox{.45\ht0}{\textcolor{#1}{\rule{\wd0}{1pt}}}}#2}

%\usetheme{Berlin}
%\usecolortheme{seahorse}
%\usefonttheme{professionalfonts}

\begin{document}

  \subsection*{Solution to Homework 1}

  \begin{enumerate}
	\item $H$ is symmetric, i.e.~$H^\top = H$:
	\begin{align*}
	H^\top &= \left( X(X^\top X)^{-1}X^\top \right)^\top & {\color{red} \left\{ (ABC)^\top = C^\top B^\top A^\top \right\}}\\
	 &= \left(X^\top\right)^\top \left((X^\top X)^{-1}\right)^\top X^\top & {\color{red} \left\{ (A^\top)^\top = A, (A^{-1})^\top = (A^\top)^{-1} \right\}}\\
	 &= X \left((X^\top X)^\top\right)^{-1} X^\top & {\color{red} \left\{ (AB)^\top = B^\top A^\top \right\}}\\
	 &= X \left(X^\top \left(X^\top\right)^\top\right)^{-1} X^\top & {\color{red} \left\{ (A^\top)^\top = A \right\}}\\
	 &= X (X^\top X)^{-1} X^\top = H.
	\end{align*}
	\item $H$ is idempotent, i.e.~$H^2 = HH = H$:
	\begin{align*}
	H^2 &= HH\\
	 &= X{\color{red} (X^\top X)^{-1}X^\top X}(X^\top X)^{-1}X^\top & {\color{red} \left\{ A^{-1} A = I \right\}}\\
	 &= {\color{red} XI}(X^\top X)^{-1}X^\top & {\color{red} \left\{ AI = A \right\}}\\
	 &= X(X^\top X)^{-1}X^\top = H.
	\end{align*}
	\item $I-H$ is idempotent, i.e.~$(I-H)^2 = (I-H)(I-H) = (I-H)$:
	\begin{align*}
	(I-H)^2 &= (I-H)(I-H)\\
	 &= II - IH - HI + HH & {\color{red} \left\{ IA = A, AI = A, HH = H \right\}}\\
	 &= I - H {\color{red} - H + H} = I - H.
	\end{align*}
  \end{enumerate}

\end{document}
